\input{../../doc}
\input{../../preamb}
\begin{document}
\subsection*{Kapittel \ref{Derivasjon}}
\footnotesize
\opr{dmhpx} \textbf{a)} $f'(x)= \frac{12}{\cos^2(4x)} $ \textbf{b)} $f'(x)= -e^{-4 x} (\sin x + 4 \cos x) $ \textbf{c)} $ f'(x)=2(\sin^2 x -\cos^2 x) $ \\\textbf{d)} $f'(x)= \frac{1}{2\tan^\frac{1}{2}x\cos^2 x} $ \textbf{e)} $f'(x)= e^{2x}\left(2\ln x +\frac{1}{x}\right) $ \textbf{f)} $ f'(x)=\frac{x \ln(x) \cos x - \sin x}{x \ln^2 x} $

\opr{vislncosx} 
\textbf{a)} Se løsningsforslag.
\textbf{b)} Se løsningsforslag.

\opr{xexpx} \textbf{a)} $ x=-1 $ og $ x=1 $ \textbf{b)} $ f(-1)=-e $ og $ f(1)=e^{-1} $

\opr{vendepkt} \textbf{a)} Se løsningsforslag. \textbf{b)} $ x = \frac{1}{2k}(\pi+4\pi n + 2c) $

\opr{antideropg} \textbf{a)} Fordi $ F'(x)=f(x) $. \textbf{b)} Fordi  $ F'(x)=f(x) $. 
\end{document}